book/FPLean/HelloWorld/StepByStep.lean
@@ -7,6 +7,7 @@ open Verso.Genre Manual
 open FPLean
 
 set_option verso.exampleProject "../examples"
+set_option verso.exampleModule "HelloName"
 
 example_module Examples.HelloWorld
 
@@ -15,10 +16,10 @@ example_module Examples.HelloWorld
 #doc (Manual) "Step By Step" =>
 
 :::paragraph
-A {moduleTerm HelloName}`do` block can be executed one line at a time.
+A {moduleTerm}`do` block can be executed one line at a time.
 Start with the program from the prior section:
 
-```module HelloName (anchor:=block1)
+```anchor block1
   let stdin ← IO.getStdin
   let stdout ← IO.getStdout
   stdout.putStrLn "How would you like to be addressed?"
@@ -31,8 +32,8 @@ Start with the program from the prior section:
 # Standard IO
 
 :::paragraph
-The first line is {module (anchor:=line1)}`HelloName`, while the remainder is:
-```module HelloName (anchor:=block2)
+The first line is {anchor line1}`HelloName`, while the remainder is:
+```anchor block2
   let stdout ← IO.getStdout
   stdout.putStrLn "How would you like to be addressed?"
   let input ← stdin.getLine
@@ -41,22 +42,22 @@ The first line is {module (anchor:=line1)}`HelloName`, while the remainder is:
 ```
 :::
 
-To execute a {kw}`let` statement that uses a `←`, start by evaluating the expression to the right of the arrow (in this case, {moduleTerm HelloName}`IO.getStdin`).
+To execute a {kw}`let` statement that uses a `←`, start by evaluating the expression to the right of the arrow (in this case, {moduleTerm}`IO.getStdin`).
 Because this expression is just a variable, its value is looked up.
-The resulting value is a built-in primitive {moduleTerm HelloName}`IO` action.
-The next step is to execute this {moduleTerm HelloName}`IO` action, resulting in a value that represents the standard input stream, which has type {moduleTerm HelloName}`IO.FS.Stream`.
-Standard input is then associated with the name to the left of the arrow (here {moduleTerm HelloName (anchor:=line1)}`stdin`) for the remainder of the {moduleTerm HelloName}`do` block.
+The resulting value is a built-in primitive {moduleTerm}`IO` action.
+The next step is to execute this {moduleTerm}`IO` action, resulting in a value that represents the standard input stream, which has type {moduleTerm}`IO.FS.Stream`.
+Standard input is then associated with the name to the left of the arrow (here {anchorTerm line1}`stdin`) for the remainder of the {moduleTerm}`do` block.
 
-Executing the second line, {module (anchor:=line2)}`HelloName`, proceeds similarly.
-First, the expression {moduleTerm HelloName}`IO.getStdout` is evaluated, yielding an {moduleTerm HelloName}`IO` action that will return the standard output.
+Executing the second line, {anchor line2}`HelloName`, proceeds similarly.
+First, the expression {moduleTerm}`IO.getStdout` is evaluated, yielding an {moduleTerm}`IO` action that will return the standard output.
 Next, this action is executed, actually returning the standard output.
-Finally, this value is associated with the name {moduleTerm HelloName (anchor:=line2)}`stdout` for the remainder of the {moduleTerm HelloName}`do` block.
+Finally, this value is associated with the name {anchorTerm line2}`stdout` for the remainder of the {moduleTerm}`do` block.
 
 # Asking a Question
 
 :::paragraph
-Now that {moduleTerm HelloName (anchor:=line1)}`stdin` and {moduleTerm HelloName (anchor:=line2)}`stdout` have been found, the remainder of the block consists of a question and an answer:
-```module HelloName (anchor:=block3)
+Now that {anchorTerm line1}`stdin` and {anchorTerm line2}`stdout` have been found, the remainder of the block consists of a question and an answer:
+```anchor block3
   stdout.putStrLn "How would you like to be addressed?"
   let input ← stdin.getLine
   let name := input.dropRightWhile Char.isWhitespace
@@ -64,33 +65,33 @@ Now that {moduleTerm HelloName (anchor:=line1)}`stdin` and {moduleTerm HelloName
 ```
 :::
 
-The first statement in the block, {module (anchor:=line3)}`HelloName`, consists of an expression.
+The first statement in the block, {anchor line3}`HelloName`, consists of an expression.
 To execute an expression, it is first evaluated.
-In this case, {moduleTerm HelloName}`IO.FS.Stream.putStrLn` has type {moduleTerm HelloName}`IO.FS.Stream → String → IO Unit`.
-This means that it is a function that accepts a stream and a string, returning an {moduleTerm HelloName}`IO` action.
+In this case, {moduleTerm}`IO.FS.Stream.putStrLn` has type {moduleTerm}`IO.FS.Stream → String → IO Unit`.
+This means that it is a function that accepts a stream and a string, returning an {moduleTerm}`IO` action.
 The expression uses [accessor notation](../getting-to-know/structures.md#behind-the-scenes) for a function call.
 This function is applied to two arguments: the standard output stream and a string.
-The value of the expression is an {moduleTerm HelloName}`IO` action that will write the string and a newline character to the output stream.
-Having found this value, the next step is to execute it, which causes the string and newline to actually be written to {moduleTerm HelloName (anchor:=setup)}`stdout`.
+The value of the expression is an {moduleTerm}`IO` action that will write the string and a newline character to the output stream.
+Having found this value, the next step is to execute it, which causes the string and newline to actually be written to {anchorTerm setup}`stdout`.
 Statements that consist only of expressions do not introduce any new variables.
 
-The next statement in the block is {module (anchor:=line4)}`HelloName`.
-{moduleTerm HelloName}`IO.FS.Stream.getLine` has type {moduleTerm HelloName}`IO.FS.Stream → IO String`, which means that it is a function from a stream to an {moduleTerm HelloName}`IO` action that will return a string.
+The next statement in the block is {anchor line4}`HelloName`.
+{moduleTerm}`IO.FS.Stream.getLine` has type {moduleTerm}`IO.FS.Stream → IO String`, which means that it is a function from a stream to an {moduleTerm}`IO` action that will return a string.
 Once again, this is an example of accessor notation.
-This {moduleTerm HelloName}`IO` action is executed, and the program waits until the user has typed a complete line of input.
+This {moduleTerm}`IO` action is executed, and the program waits until the user has typed a complete line of input.
 Assume the user writes "`David`".
-The resulting line (`"David\n"`) is associated with {moduleTerm HelloName (anchor:=block5)}`input`, where the escape sequence `\n` denotes the newline character.
+The resulting line (`"David\n"`) is associated with {anchorTerm block5}`input`, where the escape sequence `\n` denotes the newline character.
 
-```module HelloName (anchor:=block5)
+```anchor block5
   let name := input.dropRightWhile Char.isWhitespace
   stdout.putStrLn s!"Hello, {name}!"
 ```
 
 :::paragraph
-The next line, {module (anchor:=line5)}`HelloName`, is a {kw}`let` statement.
+The next line, {anchor line5}`HelloName`, is a {kw}`let` statement.
 Unlike the other {kw}`let` statements in this program, it uses `:=` instead of `←`.
-This means that the expression will be evaluated, but the resulting value need not be an {moduleTerm HelloName}`IO` action and will not be executed.
-In this case, {moduleTerm HelloName}`String.dropRightWhile` takes a string and a predicate over characters and returns a new string from which all the characters at the end of the string that satisfy the predicate have been removed.
+This means that the expression will be evaluated, but the resulting value need not be an {moduleTerm}`IO` action and will not be executed.
+In this case, {moduleTerm}`String.dropRightWhile` takes a string and a predicate over characters and returns a new string from which all the characters at the end of the string that satisfy the predicate have been removed.
 For example,
 
 {exampleIn dropBang}
@@ -108,36 +109,36 @@ yields
 {exampleInfo dropNonLetter}
 
 in which all non-alphanumeric characters have been removed from the right side of the string.
-In the current line of the program, whitespace characters (including the newline) are removed from the right side of the input string, resulting in {moduleTerm Examples.HelloWorld}`"David"`, which is associated with {moduleTerm HelloName (anchor:=block5)}`name` for the remainder of the block.
+In the current line of the program, whitespace characters (including the newline) are removed from the right side of the input string, resulting in {moduleTerm (module := Examples.HelloWorld)}`"David"`, which is associated with {anchorTerm block5}`name` for the remainder of the block.
 :::
 
 # Greeting the User
 
 :::paragraph
-All that remains to be executed in the {moduleTerm HelloName}`do` block is a single statement:
-```module HelloName (anchor:=line6)
+All that remains to be executed in the {moduleTerm}`do` block is a single statement:
+```anchor line6
   stdout.putStrLn s!"Hello, {name}!"
 ```
 :::
 
-The string argument to {moduleTerm HelloName (anchor:=line6)}`putStrLn` is constructed via string interpolation, yielding the string {moduleTerm Examples.HelloWorld}`"Hello, David!"`.
-Because this statement is an expression, it is evaluated to yield an {moduleTerm HelloName}`IO` action that will print this string with a newline to standard output.
-Once the expression has been evaluated, the resulting {moduleTerm HelloName}`IO` action is executed, resulting in the greeting.
+The string argument to {anchorTerm line6}`putStrLn` is constructed via string interpolation, yielding the string {moduleTerm (module := Examples.HelloWorld)}`"Hello, David!"`.
+Because this statement is an expression, it is evaluated to yield an {moduleTerm}`IO` action that will print this string with a newline to standard output.
+Once the expression has been evaluated, the resulting {moduleTerm}`IO` action is executed, resulting in the greeting.
 
 # `IO` Actions as Values
 
-In the above description, it can be difficult to see why the distinction between evaluating expressions and executing {moduleTerm HelloName}`IO` actions is necessary.
+In the above description, it can be difficult to see why the distinction between evaluating expressions and executing {moduleTerm}`IO` actions is necessary.
 After all, each action is executed immediately after it is produced.
 Why not simply carry out the effects during evaluation, as is done in other languages?
 
 The answer is twofold.
 First off, separating evaluation from execution means that programs must be explicit about which functions can have side effects.
 Because the parts of the program that do not have effects are much more amenable to mathematical reasoning, whether in the heads of programmers or using Lean's facilities for formal proof, this separation can make it easier to avoid bugs.
-Secondly, not all {moduleTerm HelloName}`IO` actions need be executed at the time that they come into existence.
+Secondly, not all {moduleTerm}`IO` actions need be executed at the time that they come into existence.
 The ability to mention an action without carrying it out allows ordinary functions to be used as control structures.
 
 :::paragraph
-For example, the function {term}`twice.name` takes an {moduleTerm HelloName}`IO` action as its argument, returning a new action that will execute the argument action twice.
+For example, the function {term}`twice.name` takes an {moduleTerm}`IO` action as its argument, returning a new action that will execute the argument action twice.
 
 {exampleDecl twice}
 
@@ -167,10 +168,10 @@ def nTimes (action : IO Unit) : Nat → IO Unit
 :::
 
 :::paragraph
-In the base case for {moduleTerm Examples.HelloWorld}`Nat.zero`, the result is {moduleTerm Examples.HelloWorld}`pure ()`.
-The function {moduleTerm Examples.HelloWorld}`pure` creates an {moduleTerm Examples.HelloWorld}`IO` action that has no side effects, but returns {moduleTerm Examples.HelloWorld}`pure`'s argument, which in this case is the constructor for {moduleTerm Examples.HelloWorld}`Unit`.
-As an action that does nothing and returns nothing interesting, {moduleTerm Examples.HelloWorld}`pure ()` is at the same time utterly boring and very useful.
-In the recursive step, a {moduleTerm Examples.HelloWorld}`do` block is used to create an action that first executes {moduleTerm Examples.HelloWorld}`action` and then executes the result of the recursive call.
+In the base case for {moduleTerm (module := Examples.HelloWorld)}`Nat.zero`, the result is {moduleTerm (module := Examples.HelloWorld)}`pure ()`.
+The function {moduleTerm (module := Examples.HelloWorld)}`pure` creates an {moduleTerm (module := Examples.HelloWorld)}`IO` action that has no side effects, but returns {moduleTerm (module := Examples.HelloWorld)}`pure`'s argument, which in this case is the constructor for {moduleTerm (module := Examples.HelloWorld)}`Unit`.
+As an action that does nothing and returns nothing interesting, {moduleTerm (module := Examples.HelloWorld)}`pure ()` is at the same time utterly boring and very useful.
+In the recursive step, a {moduleTerm (module := Examples.HelloWorld)}`do` block is used to create an action that first executes {moduleTerm (module := Examples.HelloWorld)}`action` and then executes the result of the recursive call.
 Executing {exampleIn}`nTimes3` causes the following output:
 
 {exampleInfo nTimes3}
@@ -178,8 +179,8 @@ Executing {exampleIn}`nTimes3` causes the following output:
 :::
 
 :::paragraph
-In addition to using functions as control structures, the fact that {moduleTerm Examples.HelloWorld}`IO` actions are first-class values means that they can be saved in data structures for later execution.
-For instance, the function {moduleName Examples.HelloWorld}`countdown` takes a {moduleTerm Examples.HelloWorld}`Nat` and returns a list of unexecuted {moduleTerm Examples.HelloWorld}`IO` actions, one for each {moduleTerm Examples.HelloWorld}`Nat`:
+In addition to using functions as control structures, the fact that {moduleTerm (module := Examples.HelloWorld)}`IO` actions are first-class values means that they can be saved in data structures for later execution.
+For instance, the function {moduleName (module := Examples.HelloWorld)}`countdown` takes a {moduleTerm (module := Examples.HelloWorld)}`Nat` and returns a list of unexecuted {moduleTerm (module := Examples.HelloWorld)}`IO` actions, one for each {moduleTerm (module := Examples.HelloWorld)}`Nat`:
 
 {exampleDecl countdown}
 
@@ -188,7 +189,7 @@ For example, it can be applied to an argument, and the length of the resulting l
 
 {exampleDecl from5}
 
-This list contains six elements (one for each number, plus a {moduleTerm Examples.HelloWorld}`"Blast off!"` action for zero):
+This list contains six elements (one for each number, plus a {moduleTerm (module := Examples.HelloWorld)}`"Blast off!"` action for zero):
 
 {exampleIn from5length}
 
@@ -197,13 +198,13 @@ This list contains six elements (one for each number, plus a {moduleTerm Example
 :::
 
 :::paragraph
-The function {moduleTerm Examples.HelloWorld}`runActions` takes a list of actions and constructs a single action that runs them all in order:
+The function {moduleTerm (module := Examples.HelloWorld)}`runActions` takes a list of actions and constructs a single action that runs them all in order:
 
 {exampleDecl runActions}
 
-Its structure is essentially the same as that of {moduleName Examples.HelloWorld}`nTimes`, except instead of having one action that is executed for each {moduleName Examples.HelloWorld}`Nat.succ`, the action under each {moduleName Examples.HelloWorld}`List.cons` is to be executed.
-Similarly, {moduleName Examples.HelloWorld}`runActions` does not itself run the actions.
-It creates a new action that will run them, and that action must be placed in a position where it will be executed as a part of {moduleName Examples.HelloWorld}`main`:
+Its structure is essentially the same as that of {moduleName (module := Examples.HelloWorld)}`nTimes`, except instead of having one action that is executed for each {moduleName (module := Examples.HelloWorld)}`Nat.succ`, the action under each {moduleName (module := Examples.HelloWorld)}`List.cons` is to be executed.
+Similarly, {moduleName (module := Examples.HelloWorld)}`runActions` does not itself run the actions.
+It creates a new action that will run them, and that action must be placed in a position where it will be executed as a part of {moduleName (module := Examples.HelloWorld)}`main`:
 
 {exampleDecl main}
 
@@ -215,13 +216,13 @@ Running this program results in the following output:
 
 :::paragraph
 What happens when this program is run?
-The first step is to evaluate {moduleName Examples.HelloWorld}`main`. That occurs as follows:
+The first step is to evaluate {moduleName (module := Examples.HelloWorld)}`main`. That occurs as follows:
 
 {exampleEval evalMain}
 
-The resulting {moduleTerm Examples.HelloWorld}`IO` action is a {moduleTerm Examples.HelloWorld}`do` block.
-Each step of the {moduleTerm Examples.HelloWorld}`do` block is then executed, one at a time, yielding the expected output.
-The final step, {moduleTerm Examples.HelloWorld}`pure ()`, does not have any effects, and it is only present because the definition of {moduleTerm Examples.HelloWorld}`runActions` needs a base case.
+The resulting {moduleTerm (module := Examples.HelloWorld)}`IO` action is a {moduleTerm (module := Examples.HelloWorld)}`do` block.
+Each step of the {moduleTerm (module := Examples.HelloWorld)}`do` block is then executed, one at a time, yielding the expected output.
+The final step, {moduleTerm (module := Examples.HelloWorld)}`pure ()`, does not have any effects, and it is only present because the definition of {moduleTerm (module := Examples.HelloWorld)}`runActions` needs a base case.
 :::
 
 # Exercise
@@ -231,7 +232,7 @@ Step through the execution of the following program on a piece of paper:
 
 {exampleDecl ExMain}
 
-While stepping through the program's execution, identify when an expression is being evaluated and when an {moduleTerm Examples.HelloWorld}`IO` action is being executed.
-When executing an {moduleTerm Examples.HelloWorld}`IO` action results in a side effect, write it down.
+While stepping through the program's execution, identify when an expression is being evaluated and when an {moduleTerm (module := Examples.HelloWorld)}`IO` action is being executed.
+When executing an {moduleTerm (module := Examples.HelloWorld)}`IO` action results in a side effect, write it down.
 After doing this, run the program with Lean and double-check that your predictions about the side effects were correct.
 :::
